src/z3testgen/Lisp.fsti
@@ -1,0 +1,5 @@
+module Lisp
+
+val read_witness_from
+  (from: (unit -> ML string))
+: ML (Seq.seq int)
