src/z3testgen/Z3.fsti
@@ -1,0 +1,11 @@
+module Z3
+
+type z3 = {
+  from_z3: unit -> ML string;
+  to_z3: string -> ML unit;
+}
+
+val with_z3
+  (#a: Type)
+  (f: (z3 -> ML a))
+: ML a
